Experiment with PURE quoting

rupicola/refinements/QExp.fst
@@ -150,6 +150,56 @@ val helper_lambda : #g :env ->
 let helper_lambda #g #a f =
   fun fsG -> f (fs_tail #a fsG) (fs_hd fsG)
 
+// val wp_lambdaWP : #g :env ->
+//                 #a :Type ->
+//                 #b :Type ->
+//                 wp: _ ->
+//                 wpBody:spec_env (extend a g) b ->
+//                 spec_env g (x:a -> PURE b (wp x))
+
+// let wp_lambdaWP #g #a #b wp wpBody fsG : pure_wp (x:a -> PURE b (wp x)) =
+//   reveal_opaque (`%pure_wp_monotonic) (pure_wp_monotonic);
+//   fun (p:pure_post (x:a -> PURE b (wp x))) ->
+//     forall (f:(x:a -> PURE b (wp x))).
+//       (forall (p':pure_post b) (fsG':fs_env (extend a g)).
+//         fsG == fs_tail fsG' ==> wp (fs_hd fsG') p' ==> wpBody fsG' p' ==>  p' (f (fs_hd fsG'))
+//       ) ==>  p f
+
+val wp_lambdaWP :
+  #g :env ->
+  #a :Type ->
+  #b :Type ->
+  wp: (a -> pure_wp b) ->
+  spec_env g (x:a -> PURE b (wp x)) ->
+  spec_env (extend a g) b
+
+let wp_lambdaWP #g #a #b wp wp' fsG : pure_wp b =
+  // wp (fs_hd fsG)
+  reveal_opaque (`%pure_wp_monotonic) (pure_wp_monotonic);
+  admit () ;
+  fun (p : pure_post b) ->
+    wp (fs_hd fsG) p /\
+    (let p' : pure_post (x:a -> PURE b (wp x)) =
+      fun f -> forall (x:a). p (f x)
+    in
+    wp' (fs_tail fsG) p')
+
+
+unfold
+val helper_lambdaWP :
+  #g :env ->
+  #a :Type ->
+  #b :Type ->
+  #wp: _ ->
+  #wp': _ ->
+  fs_oexp g (x:a -> PURE b (wp x)) wp' ->
+  fs_oexp (extend a g) b (wp_lambdaWP wp wp')
+
+let helper_lambdaWP #g #a f fsG =
+  admit () ;
+  f (fs_tail #a fsG) (fs_hd fsG)
+
+
 unfold
 val helper_refv: #g:env ->
                 #a:Type ->
@@ -231,6 +281,16 @@ type compilable : #a:Type -> g:env -> wp:spec_env g a -> fs_oexp g a wp -> Type 
                               (helper_lambda f) ->
                              // (fun fsG -> f (fs_tail #a fsG) (fs_hd fsG)) ->
                 compilable g (wp_lambda #g #a #b wpBody) f
+
+| CLambdaDepWP :
+  #g :env ->
+  #a :Type ->
+  #b :Type ->
+  wp : _ ->
+  wp': _ ->
+  #f :fs_oexp g (x:a -> PURE b (wp x)) wp' ->
+  compilable #b (extend a g) (wp_lambdaWP wp wp') (helper_lambdaWP f) ->
+  compilable g wp' f
 
 | CRefinement : #g:env ->
                 #a:Type ->
@@ -336,6 +396,16 @@ let test2_if ()
 
 #pop-options
 
+unfold
+let on_true (b : bool) : Pure bool (requires b == true) (ensures fun r -> r == b) =
+  b
+
+[@@expect_failure]
+let test_on_true ()
+  : compilable_closed #(b: bool -> Pure bool (requires b == true) (ensures fun r -> r == b)) on_true
+  = let wp : bool -> pure_wp bool = _ in
+    let wp' : spec_env empty (x: bool -> PURE bool (wp x)) = fun fsG p -> True in
+    fun _ -> CLambdaDepWP #_ #bool #bool wp wp' CVar0
 
 // TODO: why do I have to hoist these outside?
 unfold
@@ -396,7 +466,7 @@ let test_always_false'' ()
   : Tot (compilable_closed always_false)
   by (norm [delta_only [`%always_false]]) // TODO: why is the unfolding necessary?
   = fun _ ->
-    CLambda (CIf CVar0 
+    CLambda (CIf CVar0
                 (CRefinement (fun y -> True) CFalse)
                 (CRefinement (fun y -> True) CVar0))
 
